code/ecdsa/Hacl.P256.fst
@@ -76,9 +76,12 @@ let compression_compressed_form b result =
 
  *)
 
-let ecp256dh_i result scalar = Hacl.Impl.EC.DH.ecp256dh_i P256 result scalar
+let ecp256dh_i_ml result scalar = Hacl.Impl.EC.DH.ecp256dh_i_ml P256 result scalar
 
-let ecp384dh_i result scalar = Hacl.Impl.EC.DH.ecp256dh_i P384 result scalar
+let ecp256dh_i_radix result scalar = Hacl.Impl.EC.DH.ecp256dh_i_radix P256 result scalar
+
+
+let ecp384dh_i result scalar = Hacl.Impl.EC.DH.ecp256dh_i_ml P384 result scalar
 
 let ecp256dh_r result pubKey scalar = Hacl.Impl.EC.DH.ecp256dh_r #P256 result pubKey scalar
 
